ocaml/eff/eff_types.ml
@@ -19,6 +19,9 @@ type ty =
   | Ty_fiberOf of ty * ty
   | Ty_union of ty * ty
   | Ty_lit of string
+  | Ty_refOf of ty
+  | Ty_deferredOf of ty * ty
+  | Ty_var of int
 
 let ctor_index_ty : ty -> int = function
   | Ty_never -> 0
@@ -37,6 +40,9 @@ let ctor_index_ty : ty -> int = function
   | Ty_fiberOf _ -> 13
   | Ty_union _ -> 14
   | Ty_lit _ -> 15
+  | Ty_refOf _ -> 16
+  | Ty_deferredOf _ -> 17
+  | Ty_var _ -> 18
 let wire_tag_ty : ty -> int = function
   | Ty_never -> 0
   | Ty_unit -> 1
@@ -54,6 +60,9 @@ let wire_tag_ty : ty -> int = function
   | Ty_fiberOf _ -> 13
   | Ty_union _ -> 14
   | Ty_lit _ -> 15
+  | Ty_refOf _ -> 16
+  | Ty_deferredOf _ -> 17
+  | Ty_var _ -> 18
 let ctor_name_ty : ty -> string = function
   | Ty_never -> "never"
   | Ty_unit -> "unit"
@@ -71,7 +80,10 @@ let ctor_name_ty : ty -> string = function
   | Ty_fiberOf _ -> "fiberOf"
   | Ty_union _ -> "union"
   | Ty_lit _ -> "lit"
-let ctor_names_ty : string list = ["never"; "unit"; "nat"; "int"; "string"; "bool"; "handle"; "option"; "list"; "prod"; "except"; "exitOf"; "causeOf"; "fiberOf"; "union"; "lit"]
+  | Ty_refOf _ -> "refOf"
+  | Ty_deferredOf _ -> "deferredOf"
+  | Ty_var _ -> "var"
+let ctor_names_ty : string list = ["never"; "unit"; "nat"; "int"; "string"; "bool"; "handle"; "option"; "list"; "prod"; "except"; "exitOf"; "causeOf"; "fiberOf"; "union"; "lit"; "refOf"; "deferredOf"; "var"]
 
 
 type lit =
